Work on ordered theorems

main.dfy
@@ -40,18 +40,22 @@ predicate ExactlyOneOf(a: bool, b: bool, c: bool) {
 // We then prove that the function is unique (NegIsUnique)
 ghost function neg(x: RR): RR
 	ensures add(x, neg(x)) == Zero
+	ensures add(neg(x), x) == Zero
 {
 	assert (exists y: RR :: add(x, y) == Zero) by {Inverse(x);}
 	var y :| add(x, y) == Zero;
+	assert add(y, x) == add(x, y) by {Conmutativity(x, y);}
 	y
 }
 
 ghost function inv(x: RR): RR
 	requires x != Zero
 	ensures mult(x, inv(x)) == One
+	ensures mult(inv(x), x) == One
 {
 	assert (exists y: RR :: mult(x, y) == One) by {Inverse(x);}
 	var y :| mult(x, y) == One;
+	assert mult(x, y) == mult(y, x) by {Conmutativity(x, y);}
 	y
 }
 
@@ -107,7 +111,7 @@ ghost function div(x: RR, y: RR): RR
 //	}
 //}
 
-lemma NegationOfNegation(x: RR)
+lemma NegOfNeg(x: RR)
 	ensures neg(neg(x)) == x
 {
 	assert add(neg(x), neg(neg(x))) == Zero; // (1)
@@ -251,6 +255,119 @@ lemma OneIsUnique(x: RR, y: RR)
 	assert mult(mult(x, y), inv(x)) == y                        by {Neutral(y);}
 }
 
+lemma NegOfSum(x: RR, y: RR)
+	ensures neg(add(x, y)) == add(neg(x), neg(y))
+{
+	assert add(add(x, y), add(neg(x), neg(y))) == add(add(y, x), add(neg(x), neg(y))) by {Conmutativity(x, y);}
+	assert add(add(x, y), add(neg(x), neg(y))) == add(y, add(x, add(neg(x), neg(y)))) by {Associativity(y, x, add(neg(x), neg(y)));}
+	assert add(add(x, y), add(neg(x), neg(y))) == add(y, add(add(x, neg(x)), neg(y))) by {Associativity(x, neg(x), neg(y));}
+	assert add(add(x, y), add(neg(x), neg(y))) == add(y, add(Zero, neg(y)))           by {Conmutativity(x, neg(x));}
+	assert add(add(x, y), add(neg(x), neg(y))) == add(y, neg(y))                      by {Conmutativity(Zero, neg(y)); Neutral(neg(y));}
+	assert add(add(x, y), add(neg(x), neg(y))) == Zero;
+
+	assert neg(add(x, y)) == add(neg(x), neg(y)) by {NegIsUnique(add(x, y), add(neg(x), neg(y)));}
+}
+
+lemma NegOfSub(x: RR, y: RR)
+	ensures neg(sub(x, y)) == sub(y, x)
+{
+	assert neg(sub(x, y)) == neg(add(x, neg(y)));
+	assert neg(sub(x, y)) == add(neg(x), neg(neg(y))) by {NegOfSum(x, neg(y));}
+	assert neg(sub(x, y)) == add(neg(x), y)           by {NegOfNeg(y);}
+	assert neg(sub(x, y)) == add(y, neg(x))           by {Conmutativity(neg(x), y);}
+	assert neg(sub(x, y)) == sub(y, x);
+}
+
+lemma NonzeroProductIsNonzero(x: RR, y: RR)
+	requires x != Zero
+	requires y != Zero
+	ensures mult(x, y) != Zero
+{
+	assert mult(inv(y), mult(x, y)) == mult(mult(x, y), inv(y)) by {Conmutativity(inv(y), mult(x, y));}
+	assert mult(inv(y), mult(x, y)) == mult(x, mult(y, inv(y))) by {Associativity(x, y, inv(y));}
+	assert mult(inv(y), mult(x, y)) == x                        by {Neutral(x);}
+
+	if mult(x, y) == Zero {
+		assert mult(inv(y), mult(x, y)) == Zero by {AnythingTimesZeroIsZero(inv(y));}
+		assert false                            by {InverseIsNeverZero(y);}
+	}
+}
+
+lemma Neutrals(x: RR)
+	ensures add(x, Zero) == x
+	ensures add(Zero, x) == x
+	ensures sub(x, Zero) == x
+	ensures sub(Zero, x) == neg(x)
+	ensures mult(x, One) == x
+	ensures mult(One, x) == x
+	ensures One != Zero
+	ensures div(x, One) == x
+	ensures x != Zero ==> div(One, x) == inv(x)
+{
+	assert One != Zero                  by {Neutral(Zero);}
+	assert add(x, Zero) == x            by {Neutral(x);}
+	assert add(Zero, x) == add(x, Zero) by {Conmutativity(x, Zero);}
+	assert mult(x, One) == x            by {Neutral(x);}
+	assert mult(One, x) == mult(x, One) by {Conmutativity(x, One);}
+
+	assert sub(x, Zero) == add(x, neg(Zero)) == add(x, Zero)                by {NegZeroIsZero();}
+	assert sub(Zero, x) == add(Zero, neg(x)) == add(neg(x), Zero) == neg(x) by {Conmutativity(neg(x), Zero); Neutral(neg(x));}
+
+	assert div(x, One) == mult(x, inv(One)) == mult(x, One) by {InvOneIsOne();}
+
+	if x != Zero {
+		assert div(One, x) == mult(One, inv(x)) == mult(inv(x), One) == inv(x) by {Conmutativity(inv(x), One); Neutral(inv(x));}
+	}
+}
+
+
+lemma InvOfProd(x: RR, y: RR)
+	requires x != Zero
+	requires y != Zero
+	ensures mult(x, y) != Zero
+	ensures inv(mult(x, y)) == mult(inv(x), inv(y))
+{
+	assert mult(x, y) != Zero by {NonzeroProductIsNonzero(x, y);}
+
+	assert mult(mult(x, y), mult(inv(x), inv(y))) == mult(mult(y, x), mult(inv(x), inv(y))) by {Conmutativity(x, y);}
+	assert mult(mult(x, y), mult(inv(x), inv(y))) == mult(y, mult(x, mult(inv(x), inv(y)))) by {Associativity(y, x, mult(inv(x), inv(y)));}
+	assert mult(mult(x, y), mult(inv(x), inv(y))) == mult(y, mult(mult(x, inv(x)), inv(y))) by {Associativity(x, inv(x), inv(y));}
+	assert mult(mult(x, y), mult(inv(x), inv(y))) == mult(y, mult(One, inv(y)))             by {Conmutativity(x, inv(x));}
+	assert mult(mult(x, y), mult(inv(x), inv(y))) == mult(y, inv(y))                        by {Conmutativity(One, inv(y)); Neutral(inv(y));}
+	assert mult(mult(x, y), mult(inv(x), inv(y))) == One;
+
+	assert inv(mult(x, y)) == mult(inv(x), inv(y)) by {InvIsUnique(mult(x, y), mult(inv(x), inv(y)));}
+}
+
+lemma NegOfProdLeft(x: RR, y: RR)
+	ensures neg(mult(x, y)) == mult(neg(x), y)
+{
+	assert add(mult(x, y), mult(neg(x), y)) == add(mult(y, x), mult(y, neg(x))) by {Conmutativity(x, y); Conmutativity(neg(x), y);}
+	assert add(mult(x, y), mult(neg(x), y)) == mult(y, add(x, neg(x)))          by {Distribuitivity(y, x, neg(x));}
+	assert add(mult(x, y), mult(neg(x), y)) == mult(y, Zero);
+	assert add(mult(x, y), mult(neg(x), y)) == Zero                             by {AnythingTimesZeroIsZero(y);}
+
+	assert mult(neg(x), y) == neg(mult(x, y))                                   by {NegIsUnique(mult(x, y), mult(neg(x), y));}
+}
+
+lemma NegOfProd(x: RR, y: RR)
+	ensures neg(mult(x, y)) == mult(neg(x), y) == mult(x, neg(y))
+{
+	assert neg(mult(x, y)) == mult(neg(x), y)  by {NegOfProdLeft(x, y);}
+
+	assert neg(mult(x, y)) == neg(mult(y, x))  by {Conmutativity(x, y);}
+	assert neg(mult(y, x)) == mult(neg(y), x)  by {NegOfProdLeft(y, x);}
+	assert mult(neg(y), x) == mult(x, neg(y))  by {Conmutativity(x, neg(y));}
+}
+
+lemma ProdOfNeg(x: RR, y: RR)
+	ensures mult(neg(x), neg(y)) == mult(x, y)
+{
+	assert mult(neg(x), neg(y)) == neg(mult(x, neg(y))) by {NegOfProd(x, neg(y));}
+	assert mult(neg(x), neg(y)) == neg(neg(mult(x, y))) by {NegOfProd(x, y);}
+	assert mult(neg(x), neg(y)) == mult(x, y)           by {NegOfNeg(mult(x, y));}
+}
+
 lemma AddOnBothSides(x: RR, a: RR, b: RR)
 	requires sub(x, a) == b
 	ensures x == add(b, a)
@@ -318,6 +435,10 @@ lemma Closure(x: RR, y: RR)
 
 
 ////////////////////////////////////// Ordered Theorems ///////////////////////////////
+ghost predicate StrictlyNegative(x: RR) {
+	!StrictlyPositive(x) && x != Zero
+}
+
 ghost predicate lt(x: RR, y: RR) {
 	StrictlyPositive(sub(y, x))
 }
@@ -334,12 +455,216 @@ ghost predicate ge(x: RR, y: RR) {
 	gt(x, y) || x == y
 }
 
+lemma ComparisonTrichotomy(x: RR, y: RR)
+	ensures ExactlyOneOf(lt(x, y), gt(x, y), x == y)
+{
+	assert ExactlyOneOf(StrictlyPositive(sub(y, x)), StrictlyPositive(neg(sub(y, x))), sub(y, x) == Zero) by {Trichotomy(sub(y, x));}
+
+	if StrictlyPositive(sub(y, x)) {
+		assert lt(x, y);
+
+		if gt(x, y) {
+			assert StrictlyPositive(sub(x, y));
+			assert !StrictlyPositive(neg(sub(y, x))) by {Trichotomy(sub(y, x));}
+			assert !StrictlyPositive(sub(x, y))      by {NegOfSub(y, x);}
+			assert false;
+		}
+	}
+	else if StrictlyPositive(neg(sub(y, x))) {
+		assert StrictlyPositive(sub(x, y)) by {NegOfSub(y, x);}
+		assert ge(x, y);
+	}
+	else if sub(y, x) == Zero {
+		assert y == add(Zero, x) by {AddOnBothSides(y, x, Zero);}
+		assert y == x            by {Conmutativity(Zero, x); Neutral(x);}
+	}
+}
+
+lemma GreaterThanZero(x: RR)
+	requires gt(x, Zero)
+	ensures StrictlyPositive(x)
+	ensures x != Zero
+	ensures StrictlyNegative(neg(x))
+	ensures lt(neg(x), Zero)
+{
+	assert StrictlyPositive(sub(x, Zero));
+	assert sub(x, Zero) == x               by {Neutrals(x);}
+	assert StrictlyPositive(x);
+	assert x != Zero                       by {Trichotomy(x);}
+
+	// Contradiction
+	if !StrictlyNegative(neg(x)) {
+		assert StrictlyPositive(neg(x)) || neg(x) == Zero;
+		if StrictlyPositive(neg(x)) {
+			assert !StrictlyPositive(x) by {Trichotomy(x);}
+			assert false;
+		}
+		else if neg(x) == Zero {
+			assert neg(neg(x)) == Zero by {NegZeroIsZero();}
+			assert x == Zero           by {NegOfNeg(x);}
+			assert false;
+		}
+	}
+
+	assert x == sub(Zero, neg(x)) by {NegOfNeg(x); Neutrals(neg(x));}
+	assert StrictlyPositive(sub(Zero, neg(x)));
+}
+
+lemma LessThanZero(x: RR)
+	requires lt(x, Zero)
+	ensures StrictlyNegative(x)
+	ensures x != Zero
+	ensures StrictlyPositive(neg(x))
+	ensures gt(neg(x), Zero)
+{
+	assert StrictlyPositive(sub(Zero, x));
+	assert sub(Zero, x) == neg(x)             by {Neutrals(x);}
+	assert StrictlyPositive(neg(x));
+
+	assert x != Zero && !StrictlyPositive(x)  by {Trichotomy(x);}
+
+	assert neg(x) == sub(neg(x), Zero)        by {Neutrals(neg(x));}
+	assert StrictlyPositive(sub(neg(x), Zero));
+}
+
+lemma ComparisonClosure(x: RR, y: RR)
+	requires gt(x, Zero)
+	requires gt(y, Zero)
+	ensures gt(mult(x, y), Zero)
+{
+	assert StrictlyPositive(x)                 by {GreaterThanZero(x);}
+	assert StrictlyPositive(y)                 by {GreaterThanZero(y);}
+	assert StrictlyPositive(mult(x, y))        by {Closure(x, y);}
+	assert mult(x, y) == sub(mult(x, y), Zero) by {Neutrals(mult(x, y));}
+
+	assert StrictlyPositive(sub(mult(x, y), Zero));
+}
+
+
+lemma IneqAddOnBothSides(x: RR, a: RR, b: RR)
+	requires lt(sub(x, a), b)
+	ensures lt(x, add(b, a))
+{
+	assert StrictlyPositive(sub(b, sub(x, a)));
+
+	assert sub(b, sub(x, a)) == add(b, neg(sub(x, a)));
+	assert sub(b, sub(x, a)) == add(b, sub(a, x))       by {NegOfSub(x, a);}
+	assert sub(b, sub(x, a)) == add(b, add(a, neg(x)));
+	assert sub(b, sub(x, a)) == add(add(b, a), neg(x))  by {Associativity(b, a, neg(x));}
+	assert sub(b, sub(x, a)) == sub(add(b, a), x)       by {Associativity(b, a, neg(x));}
+
+	assert StrictlyPositive(sub(add(b, a), x));
+}
+
+lemma IneqSubOnBothSides(x: RR, a: RR, b: RR)
+	requires lt(add(x, a), b)
+	ensures lt(x, sub(b, a))
+{
+	assert StrictlyPositive(sub(b, add(x, a)));
+
+	assert sub(b, add(x, a)) == add(b, add(neg(x), neg(a))) by {NegOfSum(x, a);}
+	assert sub(b, add(x, a)) == add(b, add(neg(a), neg(x))) by {Conmutativity(neg(x), neg(a));}
+	assert sub(b, add(x, a)) == add(add(b, neg(a)), neg(x)) by {Associativity(b, neg(a), neg(x));}
+	assert sub(b, add(x, a)) == sub(sub(b, a), x);
+
+	assert StrictlyPositive(sub(sub(b, a), x));
+}
+
+lemma IneqMultOnBothSidesPos(x: RR, a: RR, b: RR)
+	requires gt(a, Zero)
+	requires a != Zero // TODO: Remove
+	requires lt(div(x, a), b)
+	ensures lt(x, mult(b, a))
+{
+	assert StrictlyPositive(sub(b, div(x, a)));
+	assert StrictlyPositive(a) by {GreaterThanZero(a);}
+	assert StrictlyPositive(mult(sub(b, div(x, a)), a)) by {Closure(sub(b, div(x, a)), a);}
+
+	assert mult(sub(b, div(x, a)), a) == mult(add(b, neg(div(x, a))), a);
+	assert mult(sub(b, div(x, a)), a) == mult(a, add(b, neg(div(x, a))))                  by {Conmutativity(a, add(b, neg(div(x, a))));}
+	assert mult(sub(b, div(x, a)), a) == add(mult(a, b), mult(a, neg(div(x, a))))         by {Distribuitivity(a, b, neg(div(x,a)));}
+	assert mult(sub(b, div(x, a)), a) == add(mult(a, b), neg(mult(a, div(x, a))))         by {NegOfProd(a, div(x, a));}
+	assert mult(sub(b, div(x, a)), a) == add(mult(a, b), neg(mult(a, mult(x, inv(a)))));
+	assert mult(sub(b, div(x, a)), a) == add(mult(a, b), neg(mult(a, mult(inv(a), x))))   by {Conmutativity(x, inv(a));}
+	assert mult(sub(b, div(x, a)), a) == add(mult(a, b), neg(mult(mult(a, inv(a)), x)))   by {Associativity(a, inv(a), x);}
+	assert mult(sub(b, div(x, a)), a) == add(mult(a, b), neg(x))                          by {Neutrals(x);}
+	assert mult(sub(b, div(x, a)), a) == sub(mult(a, b), x);
+	assert mult(sub(b, div(x, a)), a) == sub(mult(b, a), x)                               by {Conmutativity(a, b);}
+
+	assert StrictlyPositive(sub(mult(b, a), x));
+}
+
+lemma IneqMultOnBothSidesNeg(x: RR, a: RR, b: RR)
+	requires lt(a, Zero)
+	requires a != Zero // TODO: Remove
+	requires lt(div(x, a), b)
+	ensures gt(x, mult(b, a))
+{
+	assert StrictlyPositive(sub(b, div(x, a)));
+	assert StrictlyPositive(neg(a)) by {LessThanZero(a);}
+	assert StrictlyPositive(mult(sub(b, div(x, a)), neg(a)))                           by {Closure(sub(b, div(x, a)), neg(a));}
+
+	assert mult(sub(b, div(x, a)), neg(a)) == mult(sub(div(x, a), b), a)               by {NegOfProd(sub(b, div(x, a)), a); NegOfSub(b, div(x, a));}
+	assert mult(sub(b, div(x, a)), neg(a)) == mult(a, sub(div(x, a), b))               by {Conmutativity(sub(div(x, a), b), a);}
+	assert mult(sub(b, div(x, a)), neg(a)) == add(mult(a, div(x, a)), mult(a, neg(b))) by {Distribuitivity(a, div(x, a), neg(b));}
+	assert mult(sub(b, div(x, a)), neg(a)) == add(mult(div(x, a), a), mult(a, neg(b))) by {Conmutativity(a, div(x, a));}
+	assert mult(sub(b, div(x, a)), neg(a)) == add(x, mult(a, neg(b)))                  by {Associativity(x, inv(a), a); Neutrals(x);}
+	assert mult(sub(b, div(x, a)), neg(a)) == add(x, neg(mult(a, b)))                  by {NegOfProd(a, b);}
+	assert mult(sub(b, div(x, a)), neg(a)) == sub(x, mult(a, b));
+	assert mult(sub(b, div(x, a)), neg(a)) == sub(x, mult(b, a))                       by {Conmutativity(a, b);}
+
+	assert StrictlyPositive(sub(x, mult(a, b)));
+}
+
+function square(x: RR): RR {mult(x, x)}
+
+lemma SquaresNonnegative(x: RR)
+	ensures ge(square(x), Zero)
+{
+	assert ExactlyOneOf(lt(x, Zero), gt(x, Zero), x == Zero) by {ComparisonTrichotomy(x, Zero);}
+
+	if x == Zero {
+		assert mult(x, x) == Zero by {AnythingTimesZeroIsZero(Zero);}
+		assert ge(Zero, Zero);
+	}
+	else if gt(x, Zero) {
+		assert gt(mult(x, x), Zero) by {ComparisonClosure(x, x);}
+	}
+	else if le(x, Zero) {
+		assert gt(neg(x), Zero)                   by {LessThanZero(x);}
+		assert gt(mult(neg(x), neg(x)), Zero)     by {ComparisonClosure(neg(x), neg(x));}
+		assert mult(neg(x), neg(x)) == mult(x, x) by {ProdOfNeg(x, x);}
+	}
+}
+
+lemma OneIsPositive()
+	ensures ge(One, Zero)
+	ensures StrictlyPositive(One)
+{
+	assert One == square(One)    by {Neutrals(One);}
+	assert ge(square(One), Zero) by {SquaresNonnegative(One);}
+	assert One != Zero           by {Neutrals(One);}
+	assert gt(One, Zero);
+
+	assert StrictlyPositive(sub(One, Zero));
+	assert sub(One, Zero) == One by {Neutrals(One);}
+}
+
+ghost function OneAsAPositive(): RR
+	ensures StrictlyPositive(One)
+{
+	assert StrictlyPositive(One) by {OneIsPositive();}
+	One
+}
+
+// type RRPA = x: RR | StrictlyPositive(x) ghost witness OneAsAPositive()
+
 /////////////////////////////////////// Complete axioms ////////////////////////////////
 ghost predicate IsAnUpperBound(s: iset<RR>, M: RR) {
 	forall x :: x in s ==> le(x, M)
 }
 
-ghost predicate SupBound(s: iset<RR>) {
+ghost predicate UpperBounded(s: iset<RR>) {
 	exists M: RR :: IsAnUpperBound(s, M)
 }
 
@@ -347,7 +672,7 @@ ghost predicate IsALowerBound(s: iset<RR>, M: RR) {
 	forall x :: x in s ==> ge(x, M)
 }
 
-ghost predicate InfBound(s: iset<RR>) {
+ghost predicate LowerBounded(s: iset<RR>) {
 	exists M: RR :: IsALowerBound(s, M)
 }
 
@@ -360,7 +685,22 @@ ghost predicate IsTheInfimum(s: iset<RR>, M: RR) {
 }
 
 lemma SupremumExists(s: iset<RR>)
+	requires exists x :: x in s
+	requires UpperBounded(s)
 	ensures {:axiom} exists M: RR :: IsTheSupremum(s, M)
 
 
 ///////////////////////////////////// Complete Theorems ////////////////////////////////
+lemma SqrtExists(x: RR)
+	requires ge(x, Zero)
+	ensures exists y :: (ge(y, Zero) && square(y) == x)
+{
+	var numbersLessThan := iset r: RR | le(square(r), x);
+
+	assert Zero in numbersLessThan by {
+		assert square(Zero) == Zero by {AnythingTimesZeroIsZero(Zero);}
+		assert le(Zero, x); // <=> ge(x, Zero)
+	}
+
+	assume {:axiom} exists y :: (ge(y, Zero) && square(y) == x);
+}
